Work on linking simulations

sepcomp/linking.v
@@ -1,131 +1,701 @@
+Add LoadPath "..".
 Require Import sepcomp.extspec.
 Require Import sepcomp.Address.
 Require Import sepcomp.core_semantics.
+Require Import sepcomp.effect_semantics.
 Require Import sepcomp.step_lemmas.
-Require Import sepcomp.forward_simulations.
+Require Import sepcomp.mem_lemmas.
+Require Import sepcomp.effect_simulations.
 
-Require Import compcert.common.AST. (*for typ*)
-Require Import compcert.common.Values. (*for val*)
-Require Import compcert.lib.Integers.
+Require Import sepcomp.pos.
+Require Import sepcomp.stack.
 
+Require Import ssreflect ssrbool ssrnat ssrfun eqtype seq fintype finfun.
 Set Implicit Arguments.
 
-Definition runnable {G C M} (csem: CoreSemantics G C M) (c: C) :=
-  match at_external csem c, halted csem c with 
-  | None, None => true
-  | _, _ => false
-  end.
+(*NOTE: because of redefinition of [val], these imports must appear 
+  after Ssreflect eqtype.*)
+Require Import compcert.common.AST.    (*for typ*)
+Require Import compcert.common.Values. (*for val*)
+Require Import compcert.common.Globalenvs. 
+Require Import compcert.lib.Integers.
 
-Module Extension. Section Extension. 
-Variables
- (M                                (** memories *)
-  Z                                (** external states *)
-  Zint                             (** portion of Z implemented by extension *)
-  Zext                             (** portion of Z external to extension *)
-  G                                (** global environments of extended semantics *)
-  xT : Type)                       (** corestates of extended semantics *)
- (esem: CoreSemantics G xT M)      (** extended semantics *)
- (gT                               (** global environment of core semantics *)
-  cT : Type)                       (** corestates of core semantics *)
- (csem: CoreSemantics gT cT M).    (** core semantics *)
+Require Import ZArith.
+
+(** file: linking.v
+
+This file gives the operational semantics of multi-language linking
+via a functor [CoreLinker (Csem : CORESEM)].  [CoreLinker] defines the 
+following types/modules:
+
+  -[Static.t]: the type of compile-time semantics corresponding to a particular 
+  translation unit, written in a particular programming language and w/ a 
+  particular statically allocated initial global environment
+
+  -[Core.t]: Runtime states corresponding to dynamic invocations of [Static.t]s, 
+  initialized from a [Static] module to handle a particular external function 
+  call made by another [Core]
+
+  -[CallStack.t]: just lists of [Core.t]s satisfying a few well-formedness 
+  properties 
+
+  -[Linker.t]: The type of linker corestates.  Linker states contain:
+     =[cores], a function from module id's ('I_N, or integers in the range [0..N-1]) 
+      to genvs and core semantics 
+     =[fn_tbl], a table mapping external function id's to module id's, and
+     =[stack], a callstack used to maintain a stack of cores at runtime. 
+  Above, parameter [N] is the number of static modules in the program. 
+
+  -[LinkerSem]: defines the actual linking semantics. In later parts of the 
+  file, the [LinkerSem] semantics is shown to be both a [CoopCoreSem] and an 
+  [EffectSem] (cf. core_semantics.v, effect_semantics.v).
+*)
+
+(** Dummy signatures, external functions, and core semantics *)
+
+Module Dummy.
+
+Definition sig := mksignature [::] None.
+
+Definition ef  := EF_external xH sig.
+
+Program Definition coreSem {G C M: Type} : @CoreSemantics G C M :=
+  Build_CoreSemantics G C M
+    (fun _ _ _ => None)
+    (fun _ => Some (ef, sig, [::]))
+    (fun _ _ => None)
+    (fun _ => None)
+    (fun _ _ _ _ _ => False)
+    _ _ _ _.
+Next Obligation. by []. Qed.
+
+Program Definition coopSem {G C: Type} : @CoopCoreSem G C :=
+  Build_CoopCoreSem G C (@coreSem G C Memory.mem) _.
+Next Obligation. by []. Qed.
+
+Program Definition effSem {G C: Type} : @EffectSem G C :=
+  Build_EffectSem G C (@coopSem G C) (fun _ _ _ _ _ _ => False) _ _ _.
+Next Obligation. by []. Qed.
+Next Obligation. by []. Qed.
+
+Axiom genv: forall {F V}, Genv.t F V. (*FIXME*)
+
+End Dummy.
+
+Module Type CORESEM.
+Axiom M : Type. (*memories*)
+Axiom t : forall (G C: Type), Type.
+Axiom dummy : forall {G C}, t G C.
+Declare Instance instance {G C: Type} `{T : t G C} : @Coresem.t G C M.
+End CORESEM.
+
+(** * Linking semantics *)
+
+(** The [CoreLinker] module gives the operational semantics of linking. 
+    It is parameterized by a core semantics [Csem]. *)
+
+Module CoreLinker (Csem : CORESEM).
+
+(** Static semantics of translation units *)
+
+Module Static. 
+
+Record t := mk
+  { F   : Type
+  ; V   : Type
+  ; ge  : Genv.t F V
+  ; C   : Type
+  ; coreSem : Csem.t (Genv.t F V) C
+  ; init : C
+  }.
+
+Definition dummy := @mk unit unit Dummy.genv unit Csem.dummy tt.
+
+End Static.
+
+(** [Cores] are runtime execution units. *)
+
+Module Core. Section core.
+
+Variable N : pos.
+Variable cores : 'I_N -> Static.t.
+
+Import Static.
+
+Record t := mk
+  { i  : 'I_N
+  ; c  :> (cores i).(C)
+  }.
+
+Definition upd (core : t) (newC : (cores core.(i)).(C)) :=
+  {| i := core.(i)
+   ; c := newC 
+  |}.
+
+Definition dummy : t := mk (i0 N) (cores (i0 N)).(init).
+
+End core. End Core.
+
+Arguments Core.t {N} cores.
+
+Arguments Core.dummy {N} cores. 
+
+(** Linking semantics invariants: 
+    -All cores except the topmost one are at_external. 
+    -The call stack always contains at least one core. *)
+
+Import Coresem.
+
+Section coreDefs.
+
+Import Static.
+
+Variable N : pos.
+Variable cores : 'I_N -> Static.t.
+
+Definition atExternal (c: Core.t cores) :=
+  let: (Core.mk i c) := c in
+  let: F := (cores i).(F) in
+  let: V := (cores i).(V) in
+  let: C := (cores i).(C) in
+  let: coreSem := (cores i).(coreSem) in
+  if @at_external (Genv.t F V) C Csem.M (Csem.instance (T:=coreSem)) c is 
+    Some (ef, dep_sig, args) then true
+  else false.
+
+Definition wf_callStack (stk: Stack.t (Core.t cores)) :=
+  [&& all atExternal (pop stk) & size stk > 0].
+
+End coreDefs.
+
+Arguments atExternal {N} cores c.
+
+(** Call stacks are [stack]s satisfying the [wf_callStack] invariant. *)
+
+Module CallStack. Section callStack.
+
+Context {N : pos} (cores : 'I_N -> Static.t).
+
+Record t : Type := mk
+  { callStack :> Stack.t (Core.t cores)
+  ; _         :  wf_callStack callStack 
+  }.
+
+Program Definition singl (core: Core.t cores) := mk [:: core] _.
+
+Definition dummy := singl (Core.dummy cores).
+
+Section callStackDefs.
+
+Context (stack : t).
+
+Definition callStackSize := size stack.(callStack).
+
+Lemma callStack_wf : wf_callStack stack.
+Proof. by case: stack. Qed.
+
+Lemma callStack_ext : all (atExternal cores) (pop stack).
+Proof. by move: callStack_wf; move/andP=> [H1 H2]. Qed.
+
+Lemma callStack_size : callStackSize > 0.
+Proof. by move: callStack_wf; move/andP=> [H1 H2]. Qed.
+
+End callStackDefs. 
+
+End callStack. End CallStack.
+
+(** * [Linker.t]
+
+   The first two fields of this record are static configuration data:  
+   -[cores] is a function from module id's ('I_n, or integers in the range [0..n-1]) 
+    to genvs and core semantics, with existentially quantified core type [C]. 
+   -[fn_tbl] maps external function id's to module id's
+
+   [stack] is used to maintain a stack of cores, at runtime. 
+   Parameter [N] is the number of static modules in the program. *)
+
+Module Linker.
+
+Record t (N : pos) := mkLinker
+  { cores  : 'I_N  -> Static.t 
+  ; fn_tbl : ident -> option 'I_N
+  ; stack  : CallStack.t cores
+  }.
+
+End Linker.
+
+Import Linker.
+
+Notation linker := Linker.t.
+
+Section linkerDefs.
+
+Context {N : pos} (l : linker N).
+
+Import CallStack. (*for coercion [callStack]*)
+
+Definition dummy_linker := 
+  let: my_cores := fun _ : 'I_N => Static.dummy in
+  @mkLinker _ my_cores (fun id => None) (dummy my_cores).
+
+Section emptyLinker.
+
+Variable my_cores : 'I_N -> Static.t.
+Variable my_fun_tbl : ident -> option 'I_N.
+
+Definition empty_linker := @mkLinker _ my_cores my_fun_tbl (dummy my_cores).
+
+End emptyLinker.
+
+Definition updStack (newStack : CallStack.t l.(cores)) :=
+  {| cores  := l.(cores)
+   ; fn_tbl := l.(fn_tbl)
+   ; stack  := newStack
+  |}.
+
+(** [inContext]: The top core on the call stack has a return context *)
+
+Definition inContext (l0 : linker N) := callStackSize l0.(stack) > 1.
+
+(** [updCore]: Replace the top core on the call stack with [newCore] *)
+
+Program Definition updCore (newCore: Core.t l.(cores)) := 
+  updStack (CallStack.mk (push (pop l.(stack)) newCore) _).  
+
+Next Obligation. apply/andP; split=>/=; last by []; by apply: callStack_ext. Qed.
+
+(** [pushCore]: Push a new core onto the call stack.  
+    Succeeds only if all cores are currently at_external. *)
+
+Program Definition pushCore 
+  (newCore: Core.t l.(cores)) 
+  (_ : all (atExternal l.(cores)) l.(stack).(callStack)) := 
+  updStack (CallStack.mk (push l.(stack) newCore) _).
+
+Next Obligation. by rewrite/wf_callStack; apply/andP; split. Qed.
+
+(** [popCore]: Pop the top core on the call stack.  
+    Succeeds only if the top core is running in a return context. *)
+
+Lemma inContext_wf (stk : Stack.t (Core.t l.(cores))) : 
+  size stk > 1 -> wf_callStack stk -> wf_callStack (pop stk).
+
+Proof.
+rewrite/wf_callStack=> H1; move/andP=> [H2 H3]; apply/andP; split.
+- by apply: all_pop.
+- by move: H1 H2 H3; case: stk.
+Qed.
+
+Program Definition popCore : option (linker N) := 
+  (match inContext l as pf return (pf = inContext l -> option (linker N)) with
+    | true => fun pf => 
+        Some (updStack (CallStack.mk (pop l.(stack)) (inContext_wf _ _ _)))
+    | false => fun pf => None
+  end) Logic.eq_refl.
+
+Next Obligation. by apply: callStack_wf. Qed.
+
+Definition peekCore := peek l.(stack).
+
+Definition emptyStack := if l.(stack).(callStack) is [::] then true else false.
+
+Lemma peekCore_nempty c : peekCore = Some c -> emptyStack = false.
+Proof. by rewrite/peekCore/peek/emptyStack/StackDefs.peek; case: (callStack _). Qed.
+
+Import Static.
+
+Definition initCore (ix: 'I_N) (v: val) (args: list val) 
+  : option (Core.t l.(cores)):=
+  if @initial_core _ _ _ 
+       (Csem.instance (T:=(l.(cores) ix).(coreSem))) 
+       (l.(cores) ix).(Static.ge) 
+       v args 
+  is Some c then Some (Core.mk _ l.(cores) ix c)
+  else None.
+
+End linkerDefs.
+
+Notation ge_ty := (Genv.t unit unit).
+
+(** The linking semantics *)
+
+Module LinkerSem. Section linkerSem.
+
+Variable N : pos.  (* Number of (compile-time) modules *)
+Variable my_cores : 'I_N  -> Static.t.
+Variable my_fn_tbl: ident -> option 'I_N.
+
+(** [handle id l args] looks up function id [id] in function table [l.fn_tbl], 
+    producing an optional module index [ix : 'I_N].  The index is used to 
+    construct a new core to handle the call to function [id]. The new core 
+    is pushed onto the call stack. *)
+
+Section handle.
+
+Variables (id: ident) (l: linker N) (args: list val).
+
+Import CallStack.
+
+Definition handle :=
+  (match all (atExternal l.(cores)) l.(stack).(callStack) as pf 
+        return (pf = all (atExternal l.(cores)) l.(stack).(callStack) 
+               -> option (linker N)) with
+    | true => fun pf => 
+        if l.(fn_tbl) id is Some ix then
+        if initCore l ix (Vptr id Int.zero) args is Some c 
+          then Some (pushCore l c (Logic.eq_sym pf))
+        else None else None
+    | false => fun _ => None
+  end) Logic.eq_refl.
+
+End handle.
+
+(** Initial core *)
+
+Definition initial_core (tt: ge_ty) (v: val) (args: list val)
+  : option (linker N) :=
+  if v is Vptr id ofs then handle id (empty_linker my_cores my_fn_tbl) args 
+  else None.
+
+(** Is the running core at_external? *)
+
+Definition at_external0 (l: linker N) :=
+  let: mc := peekCore l in
+  if mc is Some c then 
+    let: ix  := c.(Core.i) in
+    let: sem := (l.(cores) ix).(Static.coreSem) in
+    let: F   := (l.(cores) ix).(Static.F) in
+    let: V   := (l.(cores) ix).(Static.V) in
+    @at_external (Genv.t F V) _ _ (Csem.instance (T:=sem)) (Core.c c) 
+  else None.
+
+(** Is the running core halted? *)
+
+Definition halted0 (l: linker N) :=
+  let: mc := peekCore l in
+  if mc is Some c then 
+    let: ix  := c.(Core.i) in
+    let: sem := (l.(cores) ix).(Static.coreSem) in
+    let: F   := (l.(cores) ix).(Static.F) in
+    let: V   := (l.(cores) ix).(Static.V) in
+    @halted (Genv.t F V) _ _ (Csem.instance (T:=sem)) (Core.c c) 
+  else None.
+
+(** Lift a running core step to linker step *)
+
+Definition corestep0 (l: linker N) (m: Csem.M) (l': linker N) (m': Csem.M) := 
+  let: mc := peekCore l in
+  if mc is Some c then 
+    let: ix  := c.(Core.i) in
+    let: sem := (l.(cores) ix).(Static.coreSem) in
+    let: F   := (l.(cores) ix).(Static.F) in
+    let: V   := (l.(cores) ix).(Static.V) in
+    let: ge  := (l.(cores) ix).(Static.ge) in
+    exists c', 
+      @corestep (Genv.t F V) _ _ (Csem.instance (T:=sem)) ge (Core.c c) m c' m'
+   /\ l' = updCore l (Core.upd c c')
+  else False.
+
+Definition fun_id (ef: external_function) : option ident :=
+  if ef is (EF_external id sig) then Some id else None.
+
+(** The linker is [at_external] whenever the top core is [at_external] and 
+    the [id] of the called external function isn't handleable by any 
+    compilation unit. *)
+
+Definition at_external (l: linker N) :=
+  if at_external0 l is Some (ef, dep_sig, args) 
+    then if fun_id ef is Some id then
+         if handle id l args is None then Some (ef, dep_sig, args) else None
+         else None
+  else at_external0 l.
+
+Definition after_external (mv: option val) (l: linker N) :=
+  let: mc := peekCore l in
+  if mc is Some c then 
+    let: ix  := c.(Core.i) in
+    let: sem := (l.(cores) ix).(Static.coreSem) in
+    let: F   := (l.(cores) ix).(Static.F) in
+    let: V   := (l.(cores) ix).(Static.V) in
+    let: ge  := (l.(cores) ix).(Static.ge) in
+      if @after_external (Genv.t F V) _ _ (Csem.instance (T:=sem)) mv (Core.c c) 
+        is Some c' then Some (updCore l (Core.upd c c'))
+      else None
+  else None.
+
+(** The linker is [halted] when the last core on the call stack is halted. *)
+
+Definition halted (l: linker N) := 
+  if ~~inContext l then 
+  if halted0 l is Some rv then Some rv
+  else None else None.
+
+(** Corestep relation of linking semantics *)
+
+Definition corestep (ge: ge_ty) (l: linker N) (m: Csem.M) (l': linker N) (m': Csem.M) := 
+  (** 1- The running core takes a step, or *)
+  corestep0 l m l' m' \/
+
+  (** 2- We're in a function call context. In this case, the running core is either *)
+  (m=m' 
+   /\ ~corestep0 l m l' m' 
+   /\ if inContext l then 
+
+      (** 3- at_external, in which case we push a core onto the stack to handle 
+         the external function call (or this is not possible because no module 
+         handles the external function id, in which case the entire linker is 
+         at_external) *)
+
+      if at_external0 l is Some (ef, dep_sig, args) then
+      if fun_id ef is Some id then
+      if handle id l args is Some l'' then l'=l'' else False else False
+      else 
+
+      (** 4- or halted, in which case we pop the halted core from the call stack
+         and inject its return value into the caller's corestate. *)
+
+      if halted0 l is Some rv then
+      if popCore l is Some l0 then 
+      if after_external (Some rv) l0 is Some l'' then l'=l'' 
+      else False else False else False
+
+     else False).
+
+Lemma corestep_not_at_external0 m c m' c' :
+  corestep0 c m c' m' -> at_external0 c = None.
+Proof.
+rewrite/corestep0/at_external0; case: (peekCore c)=>// a [newCore][H1 H2].
+by apply corestep_not_at_external in H1.
+Qed.
+
+Lemma at_external_halted_excl0 c :
+  at_external0 c = None \/ halted0 c = None.
+Proof.
+rewrite/at_external0/halted0; case: (peekCore c); last by right.
+by move=> a; apply: at_external_halted_excl.
+Qed.
+
+Lemma corestep_not_halted0 m c m' c' :
+  corestep0 c m c' m' -> halted c = None.
+Proof.
+rewrite/corestep0/halted; case Heq: (peekCore c)=>//[a].
+move=> [newCore [H1 H2]]. 
+case Hcx: (~~ inContext _)=>//; case Hht: (halted0 _)=>//.
+by move: Hht; apply corestep_not_halted in H1; rewrite/halted0 Heq H1.
+Qed.
+
+Lemma corestep_not_at_external ge m c m' c' :
+  corestep ge c m c' m' -> at_external c = None.
+Proof.
+rewrite/corestep/at_external. 
+move=> [H|[_ [_ H]]]; first by move: H; move/corestep_not_at_external0=> ->.
+move: H; case Hcx: (inContext _)=>//.
+case Heq: (at_external0 c)=>//[[[ef sig] args]].
+move: Heq; case: (at_external_halted_excl0 c)=> [H|H]; first by rewrite H.
+by move=> H2; case: (fun_id ef)=>// id; case: (handle _ _ _).
+Qed.
+
+Lemma at_external0_not_halted c x :
+  at_external0 c = Some x -> halted c = None.
+Proof.
+case: (at_external_halted_excl0 c); rewrite/at_external0/halted.
+by case Heq: (peekCore c)=>//[a] ->.
+move=> H; case Heq: (peekCore c)=>//[a]. 
+by case Hcx: (~~ inContext _)=>//; rewrite H.
+Qed.
+
+Lemma corestep_not_halted ge m c m' c' :
+  corestep ge c m c' m' -> halted c = None.
+Proof. 
+rewrite/corestep/halted.
+move=> [H|[_ [_ H]]]; first by move: H; move/corestep_not_halted0.
+by move: H; case Hcx: (inContext _).
+Qed.
+
+Lemma at_external_halted_excl c :
+  at_external c = None \/ halted c = None.
+Proof.
+rewrite/at_external/halted; case Hat: (at_external0 c)=>//; 
+first by right; apply: (at_external0_not_halted _ Hat). 
+by left.
+Qed.
+
+Lemma after_at_external_excl rv c c' :
+  after_external rv c = Some c' -> at_external c' = None.
+Proof.
+rewrite/after_external/at_external; case: (peekCore c)=>// a. 
+case Heq: (Coresem.after_external _ _)=>//.
+inversion 1; subst.
+case Hat: (at_external0 _)=>//[[[ef sig] args]].
+move: Hat; rewrite/at_external0=>/= H2.
+by apply after_at_external_excl in Heq; rewrite Heq in H2. 
+Qed.
+
+Definition coresem : CoreSemantics ge_ty (linker N) Csem.M :=
+  Build_CoreSemantics ge_ty (linker N) Csem.M 
+    initial_core
+    at_external
+    after_external
+    halted 
+    corestep
+    corestep_not_at_external    
+    corestep_not_halted 
+    at_external_halted_excl
+    after_at_external_excl.
+
+End linkerSem. End LinkerSem.
+
+End CoreLinker.
+
+(** * Build instances for CoopCoreSem, EffectSem *)
+
+Arguments core_instance {G C M} _.
+
+Instance coop_instance (G C: Type) (csem: @CoopCoreSem G C) 
+  : @Coresem.t G C Memory.mem := core_instance csem.
+
+Module Coopsem <: CORESEM.
+Definition M := Memory.mem.
+Definition t (G C: Type) := @CoopCoreSem G C.
+Definition dummy (G C: Type) := @Dummy.coopSem G C.
+Definition instance (G C: Type) (csem : t G C) := core_instance csem.
+End Coopsem.
+
+Instance effect_instance (G C: Type) (csem: @EffectSem G C) 
+  : @Coresem.t G C Memory.mem := core_instance csem.
+
+Module Effectsem <: CORESEM.
+Definition M := Memory.mem.
+Definition t (G C: Type) := @EffectSem G C.
+Definition dummy (G C: Type) := @Dummy.effSem G C.
+Definition instance (G C: Type) (csem : t G C) := effect_instance csem.
+End Effectsem.
+
+Module Linker := CoreLinker Effectsem. Import Linker.
+Module Sem    := Linker.LinkerSem.
+
+(** Specialize to effect semantics *)
+
+Section effingLinker.
+
+Variable N : pos. 
+Variable my_cores : 'I_N -> Static.t. 
+Variable my_fun_tbl : ident -> option 'I_N.
+
+Import Linker.
+
+Definition effstep0 U (l: linker N) m (l': linker N) m' := 
+  let: mc := peekCore l in
+  if mc is Some c then 
+    let: ix  := c.(Core.i) in
+    let: sem := (l.(cores) ix).(Static.coreSem) in
+    let: F   := (l.(cores) ix).(Static.F) in
+    let: V   := (l.(cores) ix).(Static.V) in
+    let: ge  := (l.(cores) ix).(Static.ge) in
+    exists c', 
+      @effstep (Genv.t F V) _ sem ge U (Core.c c) m c' m'
+    /\ l' = updCore l (Core.upd c c')
+  else False.
+
+Lemma effstep0_unchanged U l m l' m' : 
+  effstep0 U l m l' m' ->
+  Memory.Mem.unchanged_on (fun b ofs => U b ofs = false) m m'.
+Proof. 
+rewrite/effstep0; case: (peekCore l)=> // n [c'][STEP].
+by move: {STEP}(effax1 _ _ _ _ _ _ _ STEP)=> [STEP]UNCH H2.
+Qed.
+
+Lemma effstep0_corestep0 U l m l' m' : 
+  effstep0 U l m l' m' -> Sem.corestep0 l m l' m'.
+Proof. 
+rewrite/effstep0/Sem.corestep0; case: (peekCore l)=> // c0 [c'][STEP].
+move: {STEP}(effax1 _ _ _ _ _ _ _ STEP)=> [STEP]UNCH H2.
+by exists c'; split.
+Qed.
+
+Lemma effstep0_forward U l m l' m' : 
+  effstep0 U l m l' m' -> mem_forward m m'.
+Proof. 
+move/(effstep0_corestep0 _); rewrite/Sem.corestep0. 
+case: (peekCore l)=> // c0 [c'][STEP] H1. 
+by apply: {STEP}(corestep_fwd _ _ _ _ _ _ STEP). 
+Qed.
+
+Definition inner_effstep (ge: ge_ty)
+  (l: linker N) m (l': linker N) m' := 
+  [/\ Sem.corestep ge l m l' m' 
+    & Sem.corestep0 l m l' m' -> exists U, effstep0 U l m l' m'].
+
+Definition effstep (ge: ge_ty) V
+  (l: linker N) m (l': linker N) m' := 
+  [/\ Sem.corestep ge l m l' m' 
+    & Sem.corestep0 l m l' m' -> effstep0 V l m l' m'].
+
+Section csem.
+
+Notation mycsem := (Sem.coresem N my_cores my_fun_tbl).
+
+Program Definition csem : CoreSemantics ge_ty (linker N) Memory.Mem.mem := 
+  Build_CoreSemantics ge_ty (linker N) Memory.Mem.mem 
+    (initial_core mycsem)
+    (at_external mycsem)
+    (after_external mycsem)
+    (halted mycsem) 
+    inner_effstep _ _ _ _.
+
+Next Obligation. 
+move: H; rewrite/inner_effstep=> [[H1] H2]. 
+by apply: (Sem.corestep_not_at_external H1).
+Qed.
+
+Next Obligation.
+move: H; rewrite/inner_effstep=> [[H1] H2]. 
+by apply: (Sem.corestep_not_halted H1).
+Qed.
+
+Next Obligation. by apply: (Sem.at_external_halted_excl). Qed.
+Next Obligation. by apply (Sem.after_at_external_excl _ _ H). Qed.
+
+End csem.
+
+(** Reconstruct coopsem *)
+
+Program Definition coopsem := Build_CoopCoreSem _ _ csem _.
+
+Next Obligation. 
+move: CS; case; move=>[H1|[<- [H0 H1]]]. 
+by move/(_ H1)=>{H1} [U EFF]; apply (effstep0_forward _ _ _ _ EFF).
+by move=> ?; apply mem_forward_refl.
+Qed.
+
+(** Effect semantics *)
+
+Program Definition effsem := Build_EffectSem _ _ coopsem effstep _ _ _.
+
+Next Obligation. 
+move: H=>[H1]H2; split. 
+by split=> //; move=> H3; move: {H2 H3}(H2 H3)=> STEP; exists M.
+case: H1=> [H1|[<- [H0 H1]]]=> //. 
+by move: (H2 H1)=> H3; apply: (effstep0_unchanged _ _ _ _ _ H3).
+Qed.
+
+Next Obligation.
+move: H; rewrite/inner_effstep=> [[[H1|[<- [H0 H1]]]]] H2=> //.
+move: (H2 H1)=> {H2}[U H3]; exists U; split=> //.
+by left; apply: (effstep0_corestep0 _ _ _ _ _ H3).
+by exists [fun _ _ => false]; split=> //; right.
+Qed.
+
+Next Obligation.
+move: H; rewrite/effstep=>[[H1]] H2; split=> // H3; move: (H2 H3). 
+rewrite/effstep0; case: (peekCore c)=> // c0 [] x [] STEP ->.
+by move: (effstep_sub_val _ _ _ _ _ _ _ _ UV STEP)=> STEP'; exists x; split.
+Qed.
+
+End effingLinker.
 
 
-(* Signature of a linked semantics *)
 
- Record Sig := 
-   Make { proj_core: xT -> cT
-        ; proj_zint: xT -> Zint
-        ; proj_zext: Z -> Zext
-        ; zmult: Zint -> Zext -> Z
-        ; zmult_proj: forall zint zext, proj_zext (zmult zint zext)=zext
- 
-        ; zint_invar_after_external: 
-            forall ef sig args ret s s',
-            at_external esem s = Some (ef, sig, args) -> 
-            after_external esem ret s = Some s' -> proj_zint s=proj_zint s'
 
-        ; zint_invar_over_corestep: 
-            forall ge ge_core s m s' m',
-            corestep csem ge_core (proj_core s) m (proj_core s') m' ->
-            corestep esem ge s m s' m' ->
-            proj_zint s=proj_zint s'
 
-        ; handled (ef: AST.external_function) :=
-            forall (s: xT) (c: cT) sig args,
-            let c := proj_core s in
-            at_external csem c = Some (ef, sig, args) ->
-            at_external esem s = None
-
-        ; handled_invar: 
-            forall s c s' c' ef sig args sig' args',
-            proj_core s = c -> 
-            at_external csem c = Some (ef, sig, args) ->
-            at_external esem s = None -> 
-            proj_core s' = c' ->
-            at_external csem c' = Some (ef, sig', args') ->
-            at_external esem s' = None
-        }.
-
-End Extension. End Extension.
-
-Implicit Arguments Extension.Sig [M G xT].
-Implicit Arguments Extension.Make [G xT cT M Z Zint Zext].
-
-(** Core compatibility: some administrative requirements on the 
-    interactions between extensions and cores. *)
-
-Section CoreCompatible. 
-Variables
- (M                                (** memories *)
-  Z                                (** external states *)
-  Zint                             (** portion of Z implemented by extension *)
-  Zext                             (** portion of Z external to extension *)
-  G                                (** global environments of extended semantics *)
-  xT : Type)                       (** corestates of extended semantics *)
- (esem: CoreSemantics G xT M)      (** extended semantics *)
- (gT                               (** global environment of core semantics *)
-  cT : Type)                       (** corestates of core semantics *)
- (csem: CoreSemantics gT cT M).    (** core semantics *)
-
- Variables (ge: G) (geT: gT).
- Variable E: Extension.Sig Z Zint Zext esem gT cT csem.
-
- Import Extension.
-
- Inductive core_compatible: Type := CoreCompatible: forall
- (runnable_corestep: forall s m s' m',
-   let c := proj_core E s in
-   runnable csem c=true -> 
-   corestep esem ge s m s' m' -> 
-   corestep csem geT c m (proj_core E s') m')
- (** After a corestep of the inner core, the active thread's new
-    corestate is appropriately injected into the extended state. Note
-    that this condition typically imposes determinism on the inner
-    core semantics.  We can live with this because we are in general
-    dealing with deterministic semantics anyway.  To weaken the
-    determinism condition, one could make proj_core a relation, or
-    equivalently, have proj_core project a /set/ of corestates; but at
-    the current stage, the conveniences of proj_core-as-function
-    appear to outweigh the disadvantages. *)
- (corestep_pres: forall s m c' s' m' m'',
-   let c := proj_core E s in
-   corestep csem geT c m c' m' -> 
-   corestep esem ge s m s' m'' -> 
-   proj_core E s' = c' /\ m'=m'')
- (corestep_prog: forall s m c' m',
-   let c := proj_core E s in
-   corestep csem geT c m c' m' -> 
-   exists s', corestep esem ge s m s' m' /\ proj_core E s' = c')
- (at_external_proj: forall s ef sig args, 
-   at_external esem s = Some (ef, sig, args) ->
-   at_external csem (proj_core E s) = Some (ef, sig, args))
- (halted_proj: forall s, halted esem s = halted csem (proj_core E s))
- (after_ext_prog: forall s c' retv,
-   let c := proj_core E s in 
-   after_external csem retv c = Some c' -> 
-   exists s', after_external esem retv s = Some s' /\
-    proj_core E s' = c'),
- core_compatible.
-
-End CoreCompatible.
 
