sepcomp/linking_sim.v
@@ -1,0 +1,65 @@
+Require Import sepcomp.mem_lemmas.
+Require Import sepcomp.effect_simulations.
+Require Import sepcomp.pos.
+Require Import sepcomp.linking.
+
+Require Import ssreflect ssrbool ssrnat ssrfun eqtype seq fintype finfun.
+Set Implicit Arguments.
+
+Require Import compcert.common.AST.    (*for ident*)
+Require Import compcert.common.Values.   
+Require Import compcert.common.Globalenvs.   
+
+(** * Linking simulation proof 
+
+This file states and proves the main linking simulation result.
+
+*)
+
+Require Import sepcomp.wf_lemmas.
+
+Section linkingSimulation.
+
+Import SM_simulation.
+Import Linker.
+Import Static.
+
+Arguments core_data {F1 V1 C1 F2 V2 C2 Sem1 Sem2 ge1 ge2} _ _.
+Arguments core_ord  {F1 V1 C1 F2 V2 C2 Sem1 Sem2 ge1 ge2 entry_points} _ _ _.
+
+Variable N : pos.
+Variable (cores_S cores_T : 'I_N -> Static.t). 
+Variable fun_tbl : ident -> option 'I_N.
+Variable entry_points : seq (val*val*signature).
+Variable (sims : forall i : 'I_N, 
+  let s := cores_S i in
+  let t := cores_T i in
+  SM_simulation_inject s.(coreSem) t.(coreSem) s.(ge) t.(ge) entry_points).
+Variable my_ge : ge_ty.
+Variable my_ge_S : forall (i : 'I_N), genvs_domain_eq my_ge (cores_S i).(ge).
+Variable my_ge_T : forall (i : 'I_N), genvs_domain_eq my_ge (cores_T i).(ge).
+
+Let types := fun i : 'I_N => (sims i).(core_data entry_points).
+Let ords : forall i : 'I_N, types i -> types i -> Prop 
+  := fun i : 'I_N => (sims i).(core_ord).
+
+Variable wf_ords : forall i : 'I_N, well_founded (ords i).
+
+Let linker_S := effsem N cores_S fun_tbl.
+Let linker_T := effsem N cores_T fun_tbl.
+
+Let ord := @Lex.ord N types ords.
+
+Lemma link : SM_simulation_inject linker_S linker_T my_ge my_ge entry_points.
+Proof.
+
+eapply Build_SM_simulation_inject
+  with (core_data := Lex.t types)
+       (core_ord  := ord).
+
+(* well_founded ord *)
+- by apply: Lex.wf_ord.
+
+Admitted. (*WORK-IN-PROGRESS*)
+
+End linkingSimulation.
