sepcomp/pos.v
@@ -1,0 +1,9 @@
+Require Import ssreflect ssrbool ssrnat ssrfun eqtype seq fintype finfun.
+Set Implicit Arguments.
+
+Record pos := mkPos { n :> nat ; N_pos : (0 < n)%coq_nat }.
+
+Lemma is_pos (p : pos) : 0 < p.
+Proof. by case: p=> m pf; apply/ltP. Qed.
+
+Definition i0 (p : pos) : 'I_p := Ordinal (is_pos p).
