sepcomp/stack.v
@@ -1,0 +1,42 @@
+Require Import ssreflect ssrbool ssrnat ssrfun eqtype seq fintype finfun.
+Set Implicit Arguments.
+
+Module Stack.
+Definition t (T : Type) := seq T.
+End Stack.
+
+Module StackDefs. Section stackDefs.
+Variable T : Type.
+
+Import Stack.
+
+Definition updStack (newStack : seq T) := newStack.
+Definition push (stack: Stack.t T) (t: T) := updStack [:: t & stack].
+Definition peek (stack: Stack.t T) : option T :=
+  if stack is [:: topT & rest] then Some topT else None.
+Definition pop  (stack: Stack.t T) : Stack.t T := behead stack.
+Definition empty : Stack.t T := [::].
+
+Definition nonempty : pred (Stack.t T) := 
+  [pred s | if s is [::] then false else true].
+
+Lemma peek_nonempty (stack : Stack.t T) : 
+  nonempty stack -> exists t, peek stack = Some t.
+Proof. by case: stack=>// a l _; exists a. Qed.
+
+Lemma all_pop (stack : Stack.t T) p : all p stack -> all p (pop stack).
+Proof. by case: stack=>//= a l; move/andP=> [H1 H2]. Qed.
+
+End stackDefs. End StackDefs.
+
+(** Export push, pop, empty, nonempty, push_pop, pop_nonempty *)
+
+Definition push      := StackDefs.push.
+Definition pop       := StackDefs.pop.
+Definition peek      := StackDefs.peek.
+Definition empty     := StackDefs.empty.
+Definition nonempty  := StackDefs.nonempty.
+Definition peek_nonempty := StackDefs.peek_nonempty.
+Definition all_pop   := StackDefs.all_pop.
+
+Implicit Arguments empty [T].
